

## Problem Set 7, Oct 30, 2025 (Solutions to Theory Questions Part)

### Problem 1 (Kernels):

In class we have seen that many kernel functions  $k(\mathbf{x}, \mathbf{x}')$  can be written as inner products  $\phi(\mathbf{x})^\top \phi(\mathbf{x}')$ , for a suitably chosen vector-function  $\phi(\cdot)$  (often called a feature map). Let us say that such a kernel function is *valid*. We further discussed many operations on valid kernel functions that result again in valid kernel functions. Here are two more.

1. Let  $k_1(\mathbf{x}, \mathbf{x}')$  be a valid kernel function. Let  $f$  be a polynomial with positive coefficients. Show that  $k(\mathbf{x}, \mathbf{x}') = f(k_1(\mathbf{x}, \mathbf{x}'))$  is a valid kernel.
2. Show that  $k(\mathbf{x}, \mathbf{x}') = \exp(k_1(\mathbf{x}, \mathbf{x}'))$  is a valid kernel assuming that  $k_1(\mathbf{x}, \mathbf{x}')$  is a valid kernel. *Hint:* You can use the following property: if  $(K_n)_{n \geq 0}$  is a sequence of valid kernels and if there exists a function  $K : \mathcal{X} \times \mathcal{X} \rightarrow \mathbb{R}$  such that for all  $(\mathbf{x}, \mathbf{x}') \in \mathcal{X}^2$ ,  $K_n(\mathbf{x}, \mathbf{x}') \xrightarrow{n \rightarrow +\infty} K(\mathbf{x}, \mathbf{x}')$ , then  $K$  is a valid kernel.

**Solution:** *Main Idea.* For (1), we use closure of valid kernels under sums, products, and scaling by  $c \geq 0$ ; any polynomial with nonnegative coefficients is built from these operations applied to  $k_1$ , hence remains valid. For (2), we use the Taylor series  $\exp(k_1) = \lim_{n \rightarrow \infty} \sum_{i=0}^n \frac{1}{i!} k_1^i$  together with closure under pointwise limits of valid kernels.

1. • First we will prove that the sum of two valid kernels  $k_1$  and  $k_2$   $k = k_1 + k_2$  is a valid kernel. We need to construct a feature vector  $\phi(\mathbf{x})$  such that  $k(\mathbf{x}, \mathbf{x}') = \phi(\mathbf{x})^\top \phi(\mathbf{x}')$ , then by definition  $k$  would be a valid kernel.

Because kernels  $k_1$  and  $k_2$  are valid kernels

$$k_1(\mathbf{x}, \mathbf{x}') = \phi_1(\mathbf{x})^\top \phi_1(\mathbf{x}'), \quad k_2(\mathbf{x}, \mathbf{x}') = \phi_2(\mathbf{x})^\top \phi_2(\mathbf{x}'),$$

for some feature vectors  $\phi_1(\mathbf{x})$  and  $\phi_2(\mathbf{x})$ .

Lets take  $\phi(\mathbf{x}) = \begin{pmatrix} \phi_1(\mathbf{x}) \\ \phi_2(\mathbf{x}) \end{pmatrix}$ , then

$$\begin{aligned} \phi(\mathbf{x})^\top \phi(\mathbf{x}') &= (\phi_1(\mathbf{x})^\top, \phi_2(\mathbf{x})^\top) \begin{pmatrix} \phi_1(\mathbf{x}') \\ \phi_2(\mathbf{x}') \end{pmatrix} = \phi_1(\mathbf{x})^\top \phi_1(\mathbf{x}') + \phi_2(\mathbf{x})^\top \phi_2(\mathbf{x}') \\ &= k_1(\mathbf{x}, \mathbf{x}') + k_2(\mathbf{x}, \mathbf{x}') = k(\mathbf{x}, \mathbf{x}') \end{aligned}$$

Therefore  $k = k_1 + k_2$  is a valid kernel.

- Second, we will prove that the product  $k = k_1 \cdot k_2$  of two valid kernels is a valid kernel. Let's denote  $n_1$  and  $n_2$  dimensions of a feature vectors  $\phi_1(\mathbf{x})$  and  $\phi_2(\mathbf{x})$  (i.e.  $\phi_1(\mathbf{x}) \in \mathbb{R}^{n_1}$ ,  $\phi_2(\mathbf{x}) \in \mathbb{R}^{n_2}$ ).

$$k_1(\mathbf{x}, \mathbf{x}') = \sum_{i=0}^{n_1-1} \phi_{1,i}(\mathbf{x}) \phi_{1,i}(\mathbf{x}'), \quad k_2(\mathbf{x}, \mathbf{x}') = \sum_{j=0}^{n_2-1} \phi_{2,j}(\mathbf{x}) \phi_{2,j}(\mathbf{x}'),$$

Then the kernel  $k = k_1 \cdot k_2$  is

$$k(\mathbf{x}, \mathbf{x}') = \left( \sum_{i=0}^{n_1-1} \phi_{1,i}(\mathbf{x}) \phi_{1,i}(\mathbf{x}') \right) \left( \sum_{j=0}^{n_2-1} \phi_{2,j}(\mathbf{x}) \phi_{2,j}(\mathbf{x}') \right) = \sum_{i=0}^{n_1-1} \sum_{j=0}^{n_2-1} (\phi_{1,i}(\mathbf{x}) \phi_{2,j}(\mathbf{x})) (\phi_{1,i}(\mathbf{x}') \phi_{2,j}(\mathbf{x}'))$$

Lets introduce a feature vector  $\phi(\mathbf{x}) \in \mathbb{R}^{n_1 n_2}$ , such that  $\phi_{in_2+j}(\mathbf{x}) = \phi_{1,i}(\mathbf{x})\phi_{2,j}(\mathbf{x})$  for  $i \in [0, \dots, n_1 - 1], j \in [0, \dots, n_2 - 1]$ . Note that for such  $i$  and  $j$  the index of the feature vector  $\phi$  is correct:  $in_2 + j \in [0, \dots, n_1 n_2 - 1]$ . Then,

$$\begin{aligned}\phi(\mathbf{x})^\top \phi(\mathbf{x}') &= \sum_{l=0}^{n_1 n_2 - 1} \phi_l(\mathbf{x}) \phi_l(\mathbf{x}') = \sum_{i=0}^{n_1 - 1} \sum_{j=0}^{n_2 - 1} \phi_{in_2+j}(\mathbf{x}) \phi_{in_2+j}(\mathbf{x}') \\ &= \sum_{i=0}^{n_1 - 1} \sum_{j=0}^{n_2 - 1} (\phi_{1,i}(\mathbf{x}) \phi_{2,j}(\mathbf{x})) (\phi_{1,i}(\mathbf{x}') \phi_{2,j}(\mathbf{x}')) = k_1(\mathbf{x}, \mathbf{x}') \cdot k_2(\mathbf{x}, \mathbf{x}') = k(\mathbf{x}, \mathbf{x}').\end{aligned}$$

Therefore  $k(\mathbf{x}, \mathbf{x}') = k_1(\mathbf{x}, \mathbf{x}') \cdot k_2(\mathbf{x}, \mathbf{x}')$  is a valid kernel.

- Third we need to show that if  $k_1$  is a valid kernel, then  $k = c \times k_1$  with  $c \geq 0$  is also a valid kernel. Since  $k_1$  is valid, we can write for all  $x$  and  $x'$ :  $k_1(x, x') = \phi_1(x)^\top \phi_1(x')$ . Now let  $\phi(x) = \sqrt{c} \phi_1(x)$ . Notice that  $k(x, x') = c \cdot k_1(x, x') = (\sqrt{c} \phi_1(x))^\top (\sqrt{c} \phi_1(x')) = \phi(x)^\top \phi(x')$ . Hence  $c \times k_1$  is also a valid kernel.
  - Since  $f$  is only composed of the three previous operations (sum, product, multiplication by positive scalar), we can conclude that  $(x, x') \mapsto f(k_1(x, x'))$  is a valid kernel.
2. It suffices to apply the hint to the sequence of kernels  $k_n(x, x') = \sum_{i=0}^n \frac{1}{i!} k_1(x, x')^i$ . According to our previous result these are valid kernels. Since  $k_n(x, x') \xrightarrow{n \rightarrow +\infty} \exp(k_1(x, x'))$  we can apply the hint and conclude that  $k$  is a valid kernel.

**Bonus.** For the curious who are familiar with matrices and the trace operator, here is an elegant and more natural way of showing that the product of two valid kernels is a valid kernel. Notice that for  $x, x' \in \mathcal{X}^2$ :

$$\begin{aligned}k(x, x') &= k_1(x, x') \cdot k_2(x, x') \\ &= \phi_1(x)^\top \phi_1(x') \phi_2(x)^\top \phi_2(x') \\ &= \phi_1(x)^\top \phi_1(x') \phi_2(x')^\top \phi_2(x) \\ &= \text{trace}(\phi_1(x)^\top \phi_1(x') \phi_2(x')^\top \phi_2(x)) \\ &= \text{trace}(\phi_1(x') \phi_2(x')^\top \phi_2(x) \phi_1(x)^\top) \\ &= \text{trace}((\phi_2(x') \phi_1(x')^\top)^\top \phi_2(x) \phi_1(x)^\top) \\ &= \langle \phi_2(x) \phi_1(x)^\top, \phi_2(x') \phi_1(x')^\top \rangle_F\end{aligned}$$

Second equality is the definition of the valid kernels  $k_1$  and  $k_2$ , third is due to  $x^\top y = y^\top x$ , fourth is noticing that for  $z \in \mathbb{R}$   $\text{trace}(z) = z$ , fifth is that  $\text{trace}(AB) = \text{trace}(BA)$ , seventh is due to  $xy^\top = (yx^\top)^\top$ , and last is the definition of the Frobenius inner product for matrices. Hence by letting  $\phi(x) = \phi_2(x) \phi_1(x)^\top \in \mathbb{R}^{n_2 \times n_1}$  we obtain  $k(x, x') = \langle \phi(x), \phi(x') \rangle_F$ .

## Problem 2 (Softmax Cross Entropy):

In the notebook exercises we performed multiclass classification using softmax-cross-entropy as our loss. The softmax of a vector  $\mathbf{x} = [x_1, \dots, x_d]^\top$  is a vector  $\mathbf{z} = [z_1, \dots, z_d]^\top$  with:

$$z_k = \frac{\exp(x_k)}{\sum_{i=1}^d \exp(x_i)} \quad (1)$$

The label  $y$  is an integer denoting the target class. To turn  $y$  into a probability distribution for use with cross-entropy, we use one-hot encoding:

$$\text{onehot}(y) = \mathbf{y} = [y_1, \dots, y_d]^\top \text{ where } y_k = \begin{cases} 1, & \text{if } k = y \\ 0, & \text{otherwise} \end{cases} \quad (2)$$

The cross-entropy is given by:

$$H(\mathbf{y}, \mathbf{z}) = - \sum_{i=1}^d y_i \ln(z_i) \quad (3)$$

We ask you to do the following:

1. Equation 1 potentially computes  $\exp$  of large positive numbers which is numerically unstable. Modify Eq. 1 to avoid positive numbers in  $\exp$ . Hint: Use  $\max_j(x_j)$ .
2. Derive  $\frac{\partial H(\mathbf{y}, \mathbf{z})}{\partial x_j}$ . You may assume that  $\mathbf{y}$  is a one-hot vector.
3. What values of  $x_i$  minimize the softmax-cross-entropy loss? To avoid complications, practitioners sometimes use a trick called label smoothing where  $\mathbf{y}$  is replaced by  $\hat{\mathbf{y}} = (1 - \epsilon)\mathbf{y} + \frac{\epsilon}{d}\mathbf{1}$  for some small value e.g.  $\epsilon = 0.1$ .

**Solution:**

**Part 1:**

$$z_k = \frac{\exp(x_k)}{\sum_{i=1}^d \exp(x_i)} = \frac{\exp(-\max_j(x_j))}{\exp(-\max_j(x_j))} \frac{\exp(x_k)}{\sum_{i=1}^d \exp(x_i)} = \frac{\exp(x_k - \max_j(x_j))}{\sum_{i=1}^d \exp(x_i - \max_j(x_j))} \quad (4)$$

**Part 2:**

$$\begin{aligned} \frac{\partial H(\mathbf{y}, \mathbf{z})}{\partial x_j} &= \frac{\partial H(\mathbf{y}, \mathbf{z})}{\partial z_y} \frac{\partial z_y}{\partial x_j} \\ &= \frac{-1}{z_y} \frac{\partial}{\partial x_j} \frac{\exp(x_y)}{\sum_{i=1}^d \exp(x_i)} \end{aligned}$$

For  $j = y$  we have:

$$\frac{-1}{z_y} \frac{\partial}{\partial x_j} \frac{\exp(x_j)}{\sum_{i=1}^d \exp(x_i)} = -\frac{\sum_{i=1}^d \exp(x_i) \cdot \exp(x_j) \sum_{i=1}^d \exp(x_i) - \exp(x_j)^2}{\exp(x_j) (\sum_{i=1}^d \exp(x_i))^2} = -\frac{\sum_{i=1}^d \exp(x_i) - \exp(x_j)}{\sum_{i=1}^d \exp(x_i)} = z_j - 1$$

For  $j \neq y$  we have:

$$\frac{-1}{z_y} \frac{\partial}{\partial x_j} \frac{\exp(x_y)}{\sum_{i=1}^d \exp(x_i)} = -\frac{\sum_{i=1}^d \exp(x_i)}{\exp(x_y)} \cdot \frac{-\exp(x_j) \exp(x_y)}{(\sum_{i=1}^d \exp(x_i))^2} = \frac{\exp(x_j)}{\sum_{i=1}^d \exp(x_i)} = z_j$$

We can concisely write:

$$\frac{\partial H(\mathbf{y}, \mathbf{z})}{\partial \mathbf{x}} = \mathbf{z} - \mathbf{y} \quad (5)$$

**Part 3:** The optimality condition based on setting the gradient to 0 suggests that  $\mathbf{z} - \mathbf{y} = 0$ . This means that when  $j$  is equal to the correct label  $y$ , we must have  $z_j = y_j$ . Since  $z_j = \text{softmax}(\mathbf{x})_j$  and  $y_j = 1$  in this case, this implies that the following must hold:

$$\frac{e^{x_j}}{\sum_{i=1}^d e^{x_i}} = 1.$$

This can be rewritten as:

$$\frac{\sum_{i=1}^d e^{x_i}}{e^{x_j}} = 1 \implies \sum_{i=1}^d e^{x_i - x_j} = 1 \implies e^{x_j - x_j} + \sum_{i \neq j} e^{x_i - x_j} = 1 \implies \sum_{i \neq j} e^{x_i - x_j} = 0.$$

From this, we conclude that for all  $i$  not equal to  $j$ , we must have  $e^{x_i - x_j} \rightarrow 0$  or, equivalently,  $x_i - x_j \rightarrow -\infty$ . This means that  $x_i \rightarrow -\infty$  (again, for all  $i$  not equal to  $j$ , i.e., for  $i \neq y$ ) and  $x_j \rightarrow \infty$  as suggested in the solution. Also, one can verify that this solution is also consistent with the optimality of  $x_j$  for  $j \neq y$ . Thus, we conclude that the loss is minimized when  $x_j \rightarrow \begin{cases} \infty & \text{for } j = y \\ -\infty & \text{else} \end{cases}$ .

Note that the expression  $\frac{\partial H(\mathbf{y}, \mathbf{z})}{\partial \mathbf{x}} = \mathbf{z} - \mathbf{y}$  is true only if  $\mathbf{y}$  is a one-hot vector. With label smoothing,  $\mathbf{y}$  becomes a "smoothed" version of the one-hot vector, and thus we would first need to derive a different expression for the derivative of the cross-entropy loss. After doing that, it should become apparent that the optimal softmax values  $\mathbf{z}$  shouldn't be a one-hot vector anymore which will correspond to a finite minimum in terms of  $\mathbf{x}$ . Thus, the main effect of label smoothing is that it makes the minimum finite.